proof/DDC/Language/SimplePCFa/Frame.v
@@ -1,9 +1,78 @@
 
+Require Import DDC.Language.SimplePCFa.Step.
+Require Import DDC.Language.SimplePCFa.ExpSubst.
 Require Import DDC.Language.SimplePCFa.Exp.
 
 
 (* Frame stacks *)
-Definition frame := list exp.
-Hint Unfold frame.
+(* Holds the continuation while a 'let' expression reduces the bound term. *)
+Inductive frame : Set :=
+ | F : forall (t : ty) (x : exp), frame.
+Hint Constructors frame.
 
+Definition stack := list frame.
+Hint Unfold stack.
+
+
+(* Termination of an expression reduction in some context. *)
+Inductive TERMS : stack -> exp -> Prop :=
+ (* A value in an empty context has terminated. *)
+ | RfVal 
+   :  forall v
+   ,  TERMS nil (XVal v)
+
+ | RfLetPush
+   :  forall f t1 x1 x2
+   ,  TERMS (f :> F t1 x2) x1
+   -> TERMS f (XLet t1 x1 x2)
+
+ | RfLetPop
+   :  forall f t1 v1 x2
+   ,  TERMS f (substVX 0 v1 x2)
+   -> TERMS (f :> F t1 x2) (XVal v1)
+
+ | RfStep
+   :  forall f x1 x1'
+   ,  STEPP x1 x1' -> TERMS f x1'
+   -> TERMS f x1.
+Hint Constructors TERMS.
+
+
+(* Termination of an expression reduction in an empty context. *)
+Inductive TERM : exp -> Prop :=
+ | RTerm
+   : forall x
+   , TERMS nil x -> TERM x.
+Hint Constructors TERM.
+
+
+(* Wrap a frame context around an expression.
+   This converts the frame to its expression form. *)
+Fixpoint wrap (fs: stack) (x1: exp) : exp :=
+ match fs with
+ | nil           => x1
+ | f' :> F t1 x2 => wrap f' (XLet t1 x1 x2)
+ end.
+
+
+(* Reducing a term with an explicit frame is equivalent
+   to wrapping the term with its frame and reducing that. *)
+Lemma terms_wrap
+ : forall f x
+ , TERMS f x <-> TERM (wrap f x).
+Proof.
+ intros.
+ split.
+
+  intros. gen x.
+  induction f; eauto.
+   intros. induction x; simpl; destruct a; eauto.
+
+  intros. gen x.
+  induction f; intros.
+   simpl in H. inverts H. auto.
+   simpl in H. destruct a.
+    lets D: IHf H.
+    destruct x; inverts D; nope.
+Qed.  
 
